Add a crash invariant between recovery procedures
The crash invariant allows for the invariant to have held before some
wipe that resulted in the current state. This statement is automatically
derived from the refinement invariant and the semantics of crashes.

src/Refinement/Interface.v
@@ -86,11 +86,6 @@ Definition init_invariant
             fun _ w' => True;
        |}) init rec (IdRefinement world).
 
-Record crash_effect_valid `(rf: Refinement State) (wipe: State -> State) :=
-  { wipe_world_abstraction: forall w, abstraction rf (world_crash w) =
-                                 wipe (abstraction rf w);
-    wipe_idempotent: forall state, wipe (wipe state) = wipe state; }.
-
 (* Finally, an Interface ties everything together: the parameter [api] specifies all details of how the implementation behaves, while the fields give an implementation and a refinement proof.
 
 Of note is that in addition to every method being correct ([impl_ok]), the
@@ -107,13 +102,13 @@ Record Interface opT State (api: InterfaceAPI opT State) :=
                   (recover_impl interface_impl)
                   refinement;
     ret_rec_ok:
-      rec_noop (recover_impl interface_impl) refinement;
+      rec_noop (recover_impl interface_impl) refinement (crash_effect api);
     init_ok:
       init_invariant
         (init_impl interface_impl) (recover_impl interface_impl)
         refinement;
     crash_effect_ok:
-      crash_effect_valid refinement (crash_effect api); }.
+      crash_effect_valid refinement world_crash (crash_effect api); }.
 
 (* Helper function to get the implementation of a primitive operation from an
 [Interface]. *)
@@ -157,7 +152,7 @@ Definition irec opT `(api: InterfaceAPI opT State) `(i: Interface api) : prog un
   recover_impl (interface_impl i).
 
 Lemma irec_ret_ok : forall opT `(api: InterfaceAPI opT State) `(i: Interface api),
-    rec_noop (irec i) (refinement i).
+    rec_noop (irec i) (refinement i) (crash_effect api).
 Proof.
   intros.
   eapply ret_rec_ok.
@@ -236,12 +231,12 @@ Theorem crash_effect_compose : forall `(rf1: Refinement State1)
                                  `(rf2: LRefinement State1 State2)
                                  (wipe1: State1 -> State1)
                                  (wipe2: State2 -> State2),
-    crash_effect_valid rf1 wipe1 ->
+    wipe_valid rf1 wipe1 ->
     (forall state, abstraction rf2 (wipe1 state) = wipe2 (abstraction rf2 state)) ->
     (forall state, wipe2 (wipe2 state) = wipe2 state) ->
-    crash_effect_valid (refinement_compose rf1 rf2) wipe2.
+    wipe_valid (refinement_compose rf1 rf2) wipe2.
 Proof.
   intros.
   constructor; simpl; intros; eauto.
-  rewrite (wipe_world_abstraction H); eauto.
+  rewrite (wipe_abstraction H); eauto.
 Qed.
